mixfix/theorems/MixfixRepairReorder.v
@@ -100,17 +100,209 @@ Proof.
       erewrite split_last_add_last in Hrepair; eauto.
 Qed.
 
+Corollary repair_cr_start_wf g X Q t :
+  wft g X t → wft g X (repair_cr_start Q t).
+Proof.
+  intro Hwft. eapply reorder_well_formed; eauto. eapply repair_cr_start_reorder; eauto.
+Qed.
+
+Corollary repair_cr_start_preserves_yield g Q X t :
+  wft g X t → yt t = yt (repair_cr_start Q t).
+Proof.
+  intro Hwft. erewrite reorder_preserves_yield; eauto. eapply repair_cr_start_reorder; eauto.
+Qed.
+
+Lemma repair_cl_wf g p t1 ts Q :
+  wft g E (node p (cons_forest t1 ts)) → wft g E (repair_cl Q p t1 ts).
+Proof.
+  revert p ts.
+  induction t1 using parse_tree_forest_rec with
+  (P0 := fun t1s => (∀ p p1 ts,
+          wft g E (node p (cons_forest (node p1 t1s) ts)) →
+          wft g E (repair_cl_forest1 Q p p1 t1s ts)) ∧
+                    (∀ Xs p1 X1s ts ts',
+          prod g (E :: Xs) →
+          wfts g Xs ts →
+          wfts g X1s t1s →
+          repair_cl_forest2 Q (E :: Xs) p1 ts t1s = Some ts' →
+          wfts g X1s ts')); try split; intros.
+  - rename t into a.
+    cbn [repair_cl]. apply repair_cr_start_wf. assumption.
+  - rename p1 into p, p into p1, p0 into t1s.
+    simpl. apply IHt1. assumption.
+  - cbn [repair_cl_forest1]. apply repair_cr_start_wf. assumption.
+  - inv H2.
+  - rename p0 into p, t1 into t11, p into t1s.
+    cbn [repair_cl_forest1]. destruct (repair_cl_forest2 Q p p1 ts t1s) as [ts'|] eqn:?.
+    + apply IHt1.
+      inv H. inv H3. inv H4. inv H6. rename X into X11, Xs0 into X1s.
+      repeat constructor; auto.
+      eapply IHt0; eauto.
+    + apply repair_cr_start_wf. assumption.
+  - rename t1 into t11, p into t1s.
+    simpl in H2. destruct t1s as [|t12 t1s].
+    + destruct t11 as [|p11 t11s]; inv H2.
+      inv H1. inv H6. inv H5.
+      repeat constructor.
+      apply IHt1.
+      repeat constructor; auto.
+    + destruct (repair_cl_forest2 Q (E :: Xs) p1 ts (cons_forest t12 t1s)) as [t1s'|] eqn:?; inv H2.
+      inv H1. constructor; auto.
+      eapply IHt0; eauto.
+Qed.
+
+Lemma repair_cl_forest_wf g Q t1s :
+  (∀ p p1 ts,
+          wft g E (node p (cons_forest (node p1 t1s) ts)) →
+          wft g E (repair_cl_forest1 Q p p1 t1s ts)) ∧
+  (∀ Xs p1 X1s ts ts',
+          prod g (E :: Xs) →
+          wfts g Xs ts →
+          wfts g X1s t1s →
+          repair_cl_forest2 Q (E :: Xs) p1 ts t1s = Some ts' →
+          wfts g X1s ts').
+Proof.
+  induction t1s using parse_forest_tree_rec with
+  (P := fun t1 => ∀ p ts, wft g E (node p (cons_forest t1 ts)) → wft g E (repair_cl Q p t1 ts)); try split; intros.
+  - rename t into a.
+    cbn [repair_cl]. apply repair_cr_start_wf. assumption.
+  - rename p0 into p, p into p1.
+    simpl. apply IHt1s. assumption.
+  - cbn [repair_cl_forest1]. apply repair_cr_start_wf. assumption.
+  - inv H2.
+  - rename p0 into p, p into t11.
+    cbn [repair_cl_forest1]. destruct (repair_cl_forest2 Q p p1 ts t1s) as [ts'|] eqn:?.
+    + apply IHt1s.
+      inv H. inv H3. inv H4. inv H6. rename X into X11, Xs0 into X1s.
+      repeat constructor; auto.
+      eapply IHt1s0; eauto.
+    + apply repair_cr_start_wf. assumption.
+  - simpl in H2. destruct t1s as [|t12 t1s].
+    + destruct p as [|p11 t11s]; inv H2.
+      inv H1. inv H6. inv H5.
+      repeat constructor.
+      apply IHt1s.
+      repeat constructor; auto.
+    + destruct (repair_cl_forest2 Q (E :: Xs) p1 ts (cons_forest t12 t1s)) as [t1s'|] eqn:?; inv H2.
+      inv H1. constructor; auto.
+      eapply IHt1s0; eauto.
+Qed.
+
+Lemma repair_cl_preserves_yield g Q p t1 ts :
+  wft g E (node p (cons_forest t1 ts)) → yt (node p (cons_forest t1 ts)) = yt (repair_cl Q p t1 ts).
+Proof.
+  revert p ts.
+  induction t1 using parse_tree_forest_rec with 
+  (P0 := fun t1s => (∀ p p1 ts,
+                wft g E (node p (cons_forest (node p1 t1s) ts)) →
+                yt (node p (cons_forest (node p1 t1s) ts)) = yt (repair_cl_forest1 Q p p1 t1s ts)) ∧
+                    (∀ Xs p1 X1s ts t1s',
+                prod g (E :: Xs) →
+                wfts g Xs ts →
+                wfts g X1s t1s →
+                repair_cl_forest2 Q (E :: Xs) p1 ts t1s = Some t1s' →
+                yts t1s ++ yts ts = yts t1s')); try split; intros.
+  - cbn [repair_cl].
+    erewrite repair_cr_start_preserves_yield; eauto.
+  - rename p1 into p, p into p1, p0 into t1s.
+    simpl. destruct IHt1. rewrite <- H0; auto.
+  - cbn [repair_cl_forest1].
+    erewrite repair_cr_start_preserves_yield; eauto.
+  - inv H2.
+  - rename p0 into p, t1 into t11, p into t1s.
+    cbn [repair_cl_forest1]. destruct (repair_cl_forest2 Q p p1 ts t1s) as [ts'|] eqn:?.
+    + simplify_list_eq.
+      inv H. inv H3. inv H4. inv H6.
+      rewrite <- IHt1; auto.
+      destruct IHt0. erewrite H0; eauto.
+      constructor; auto. constructor; auto.
+      eapply repair_cl_forest_wf in Heqo; eauto.
+    + erewrite repair_cr_start_preserves_yield; eauto.
+  - rename t1 into t11, p into t1s.
+    simplify_list_eq. destruct t1s as [|t12 t1s].
+    + inv H1. inv H7.
+      destruct t11 as [a|p11 t11s]; inv H2.
+      simplify_list_eq. rewrite <- IHt1; auto.
+      inv H6.
+      repeat constructor; auto.
+    + simpl.
+      destruct (repair_cl_forest2 Q (E :: Xs) p1 ts (cons_forest t12 t1s)) as [t1s''|] eqn:?; inv H2.
+      simpl. destruct IHt0. inv H1. eapply H3 in Heqo; eauto. rewrite <- Heqo.
+      simplify_list_eq. reflexivity.
+Qed.
+
+Lemma repair_cl_start_wf g Q X p ts :
+  wft g X (node p ts) → wft g E (repair_cl_start Q p ts).
+Proof.
+  intro Hwft. destruct ts as [|t1 ts].
+  - simpl. inv Hwft. constructor; assumption.
+  - simpl. apply repair_cl_wf. inv Hwft. constructor; assumption.
+Qed.
+
+Lemma repair_cl_start_preserves_yield g X p ts Q :
+  wft g X (node p ts) → yt (node p ts) = yt (repair_cl_start Q p ts).
+Proof.
+  intro. destruct ts; auto.
+  simpl. inv H. erewrite <- repair_cl_preserves_yield; eauto. constructor; eauto.
+Qed.
+
+Lemma repair_wf g Q X t :
+  wft g X t → wft g X (repair Q t).
+Proof.
+  revert X. induction t using parse_tree_forest_rec with
+  (P0 := fun ts => ∀ p, wfts g p ts → wfts g p (repair_forest Q ts)); simpl; intros.
+  - assumption.
+  - inv H. eapply repair_cl_start_wf.
+    constructor; auto.
+  - assumption.
+  - inv H. constructor; auto.
+Qed.
+
+Lemma repair_forest_wf g Q ts :
+  ∀ p, wfts g p ts → wfts g p (repair_forest Q ts).
+Proof.
+  induction ts using parse_forest_tree_rec with
+  (P := fun t => ∀ X, wft g X t → wft g X (repair Q t)); simpl; intros; auto.
+  - inv H. eapply repair_cl_start_wf.
+    constructor; auto.
+  - inv H. constructor; auto.
+Qed.
+
+Lemma repair_preserves_yield g X t Q : 
+  wft g X t → yt t = yt (repair Q t).
+Proof.
+  revert X. induction t using parse_tree_forest_rec with
+  (P0 := fun ts => ∀ p, wfts g p ts → yts ts = yts (repair_forest Q ts)); intros; auto.
+  - simpl. inv H. erewrite <- repair_cl_start_preserves_yield; eauto.
+    constructor; eauto. apply repair_forest_wf; auto.
+  - simpl. inv H. erewrite <- IHt; eauto. erewrite IHt0; eauto.
+Qed. 
+
 (* Lemma repair_cl_reorder g p t1 ts Q :
   wft g E (node p (cons_forest t1 ts)) → reorder_tree (node p (cons_forest t1 ts)) (repair_cl Q p t1 ts).
 Proof.
-  intro Hwft.
-  induction t1 as [a|p1 t1s].
-  - cbn [repair_cl].
+  revert p ts.
+  induction t1 using parse_tree_forest_rec with
+  (P0 := fun t1s => (∀ p p1 ts,
+          wft g E (node p (cons_forest (node p1 t1s) ts)) →
+          reorder_tree (node p (cons_forest (node p1 t1s) ts)) (repair_cl_forest1 Q p p1 t1s ts))
+                  ∧ (∀ p p1 ts ts',
+          repair_cl_forest2 Q p p1 ts t1s = Some ts' →
+          reorder_forest_left_up p ts t1s ts')
+); try split; intros.
+  - rename t into a.
+    cbn [repair_cl].
     eapply repair_cr_start_reorder; eauto.
-  - cbn [repair_cl].
-    destruct t1s.
-    + eapply repair_cr_start_reorder; eauto.
-    + destruct (repair_cl_forest Q p p1 ts t1s) eqn:E.
-      * *)
+  - rename p1 into p, p into p1, p0 into t1s.
+    cbn [repair_cl].
+    apply IHt1; auto.
+  - cbn [repair_cl_forest1].
+    eapply repair_cr_start_reorder; eauto.
+  - inv H.
+  - rename p0 into p, t1 into t11, p into t1s.
+    cbn [repair_cl_forest1].
+    destruct (repair_cl_forest2 Q p p1 ts t1s) as [ts'|] eqn:?.
+    + apply rtc_transitive with (node p1 (cons_forest t11 ts')).
+      eapply IHt0 in Heqo. *)
 
 End MixfixRepairReorder.
